convert.js
@@ -1,0 +1,23 @@
+
+var fs = require("fs")
+var conv = require("./tofstar")
+
+var compileJSON = require("./soljson").cwrap('compileJSON', 'string', ['string', 'number']);
+
+console.log()
+
+function compile() {
+    if (process.argv.length < 3) {
+        console.err("Input file name")
+        return
+    }
+    var fname = process.argv[2]
+    var str = fs.readFileSync(fname).toString()
+    // 
+    var dta = JSON.parse(compileJSON(str))
+    var converted = conv.convertUnit(dta.sources[''].AST)
+    fs.writeFileSync(fname.replace(/\.sol/, ".fst"), converted)
+}
+
+
+compile()
