Check.fst
@@ -1,0 +1,25 @@
+module Check
+
+open FStar.All
+open FStar.UInt64
+open FStar.Heap
+
+exception Test
+
+(*
+
+let main () =
+  let i : ref UInt256.t = alloc (UInt256.uint_to_t 0) in
+  let rec loop () : ML unit = if UInt256.gt !i (UInt256.uint_to_t 100) then () else ( i := UInt256.add_mod !i (UInt256.uint_to_t 1) ; loop () ) in
+  loop ();
+  if (raise Test ; 1) + 2 = 3 then ()
+*)
+
+let test j = 
+  let i = alloc (UInt256.uint_to_t (0)) in
+  if j < 10 then raise Test;
+  let rec loop_199 () : ML unit =
+    if not (UInt256.lt (!i) (let lit : UInt256.t = UInt256.uint_to_t (10) in lit)) then () else (
+    i := UInt256.add_mod (!i) (let lit : UInt256.t = UInt256.uint_to_t (1) in lit);loop_199 ()) in
+  loop_199()
+
