Pyramid.fst
@@ -1,0 +1,154 @@
+
+(******************)
+module Pyramid
+open FStar.All
+open FStar.UInt160
+open FStar.UInt256
+open FStar.Heap
+
+type msg = {
+  sender : UInt160.t;
+  value: UInt256.t;
+}
+
+val set : #key:eqtype -> #vl:Type -> (key -> vl) -> key -> vl -> (key -> vl)
+let set #key #vl f ind x ind2 = if ind = ind2 then x else f ind2
+
+val get : #key:eqtype -> #vl:Type -> (key -> vl) -> key -> vl
+let get #key #vl f ind = f ind
+
+exception SolidityThrow
+exception SolidityReturn
+exception SolidityBadReturn
+
+val do_call : #state:Type -> #ret:Type -> (state -> ML (option ret * state)) -> state -> ML (option ret * state)
+let do_call #state #ret meth st =
+  try meth st
+  with SolidityThrow -> (None, st)
+
+val bool_and : bool -> bool -> Tot bool
+let bool_and a b = a && b
+
+val bool_or : bool -> bool -> Tot bool
+let bool_or a b = a || b
+
+(*
+
+Could generate this kind of setters and getters in methods:
+
+let balance_set addr x = s := {!s with balance = set (!s).balance addr x } in
+let balance_get addr = get (!s).balance addr in
+
+*)
+
+
+
+
+(* Storage state *)
+noeq type state = {
+parent : UInt160.t -> UInt160.t;
+balance : UInt160.t -> UInt256.t;
+invite : UInt160.t -> UInt160.t;
+invites_left : UInt160.t -> UInt256.t;
+joined : UInt160.t -> bool;
+}
+let uint256_10 = UInt256.uint_to_t (10)
+let address_0 = UInt160.uint_to_t (0)
+let uint256_1 = UInt256.uint_to_t (1)
+
+
+let uint256_0 = UInt256.uint_to_t (0)
+
+
+
+
+let uint256_3 = UInt256.uint_to_t (3)
+
+
+
+
+
+
+(* Contract methods *)
+val method_calc : msg -> state -> UInt256.t -> ML (option (UInt256.t) * state)
+let method_calc msg state level =
+let s = alloc state in
+let ret = alloc None in
+try
+ret := Some(uint256_10); raise SolidityReturn;
+(!ret, !s)
+with SolidityReturn -> (!ret, !s)
+
+
+val method_doInvite : msg -> state -> UInt160.t -> ML (option (unit) * state)
+let method_doInvite msg state addr =
+let s = alloc state in
+let ret = alloc None in
+try
+if op_disEquality (get (!s).invite (addr)) (address_0)
+then (raise SolidityThrow; ())
+else ();
+
+s := {!s with invite = set (!s).invite (addr) ((msg).sender) };
+s := {!s with invites_left = set (!s).invites_left ((msg).sender) (UInt256.sub_mod (get (!s).invites_left ((msg).sender)) (uint256_1)) };
+(!ret, !s)
+with SolidityReturn -> (!ret, !s)
+
+
+val method_cancelInvite : msg -> state -> UInt160.t -> ML (option (unit) * state)
+let method_cancelInvite msg state addr =
+let s = alloc state in
+let ret = alloc None in
+try
+if bool_or (get (!s).joined (addr)) (op_disEquality (get (!s).invite (addr)) ((msg).sender))
+then (raise SolidityThrow; ())
+else ();
+
+s := {!s with invite = set (!s).invite (addr) (address_0) };
+s := {!s with invites_left = set (!s).invites_left ((msg).sender) (UInt256.add_mod (get (!s).invites_left ((msg).sender)) (uint256_1)) };
+(!ret, !s)
+with SolidityReturn -> (!ret, !s)
+
+
+val method_pull : msg -> state -> unit -> ML (option (unit) * state)
+let method_pull msg state () =
+let s = alloc state in
+let ret = alloc None in
+try
+let sum = alloc (get (!s).balance ((msg).sender)) in
+
+s := {!s with balance = set (!s).balance ((msg).sender) (uint256_0) };
+();
+(!ret, !s)
+with SolidityReturn -> (!ret, !s)
+
+
+val method_join : msg -> state -> unit -> ML (option (unit) * state)
+let method_join msg state () =
+let s = alloc state in
+let ret = alloc None in
+try
+if UInt256.lt ((msg).value) (uint256_1)
+then (raise SolidityThrow; ())
+else ();
+
+if get (!s).joined ((msg).sender)
+then (raise SolidityThrow; ())
+else ();
+
+if bool_and (op_disEquality (get (!s).invite ((msg).sender)) (address_0)) (UInt256.gt (get (!s).invites_left (get (!s).invite ((msg).sender))) (uint256_0))
+then (let par = alloc (get (!s).invite ((msg).sender)) in
+
+s := {!s with parent = set (!s).parent ((msg).sender) (!par) };
+s := {!s with joined = set (!s).joined ((msg).sender) (true) };
+s := {!s with invites_left = set (!s).invites_left ((msg).sender) (uint256_3) };
+let i = alloc (uint256_0) in
+let rec loop_199 () : ML unit =
+if not (UInt256.lt (!i) (uint256_10)) then () else (
+s := {!s with balance = set (!s).balance (!par) (UInt256.add_mod (get (!s).balance (!par)) (let (ret,st) = method_calc msg !s
+!i in (s := st; match ret with Some x -> x | None -> (* assert False ; *) raise SolidityBadReturn))) };
+par := get (!s).parent (!par);i := UInt256.add_mod (!i) (uint256_1);loop_199 ()) in loop_199(); ())
+else ();
+
+(!ret, !s)
+with SolidityReturn -> (!ret, !s)
